Added indices in Lua + avoiding global variables

lua.v
@@ -28,53 +28,58 @@ Inductive LE : Set :=
 .
 
 
-Fixpoint Lua2Lir (Γ : IREnvironment) (e : LE) : IRE :=
+Inductive LEWT : IREnvironment -> LE -> Prop :=
+| WTNil : forall Γ, LEWT Γ LENil
+| WTNum : forall Γ n, LEWT Γ (LENum n)
+| WTPlus : forall Γ e1 e2, LEWT Γ e1 -> LEWT Γ e2 -> LEWT Γ (LEPlus e1 e2)
+| WTCnst : forall Γ, LEWT Γ LECnst
+| WTAddr : forall Γ a, LEWT Γ (LEAddr a)
+| WTGet : forall Γ e1 e2, LEWT Γ e1 -> LEWT Γ e2 -> LEWT Γ (LEGet e1 e2)
+| WTSet : forall Γ e1 e2 e3, LEWT Γ e1 -> LEWT Γ e2 -> LEWT Γ e3 ->
+               LEWT Γ (LESet e1 e2 e3)
+| WTVar : forall Γ var, In Γ var = Some IRTStar -> LEWT Γ (LEVar var)
+| WTApp : forall Γ e1 e2, LEWT Γ e1 -> LEWT Γ e2 -> LEWT Γ (LEApp e1 e2)
+| WTFun : forall Γ var body, LEWT (var |=> IRTStar; Γ) body ->
+            LEWT Γ (LEFun var body)
+.
+
+
+Fixpoint Lua2Lir (e : LE) : IRE :=
   match e with
   | LENil => IREBox TgNil IRENil
   | LENum n => IREBox TgInt (IRENum n)
-  | LEPlus e1 e2 => IREBox TgInt (IREPlus (IREUnbox TgInt (Lua2Lir Γ e1))
-                                          (IREUnbox TgInt (Lua2Lir Γ e2)))
+  | LEPlus e1 e2 => IREBox TgInt (IREPlus (IREUnbox TgInt (Lua2Lir e1))
+                                          (IREUnbox TgInt (Lua2Lir e2)))
   | LECnst => IREBox TgTbl IRECnst
-  | LEGet e1 e2 => IREGet (IREUnbox TgTbl (Lua2Lir Γ e1)) (Lua2Lir Γ e2)
-  | LESet e1 e2 e3 => IRESet (IREUnbox TgTbl (Lua2Lir Γ e1))
-                             (Lua2Lir Γ e2)
-                             (Lua2Lir Γ e3)
+  | LEGet e1 e2 => IREGet (IREUnbox TgTbl (Lua2Lir e1)) (Lua2Lir e2)
+  | LESet e1 e2 e3 => IRESet (IREUnbox TgTbl (Lua2Lir e1))
+                             (Lua2Lir e2)
+                             (Lua2Lir e3)
   | LEAddr a => IREBox TgTbl (IREAddr a)
-  | LEVar var =>
-      match In Γ var with
-      | Some _ => IREVar var
-      | None => IREBox TgNil IRENil  (* global variables are always nil *)
-      end
+  | LEVar var => IREVar var
   | LEFun var body =>
-      IREBox TgFun (IREFun
-         (IRELamb var IRTStar (Lua2Lir (var |=> IRTStar; Γ) body)))
-  | LEApp e1 e2 => IREFunApp (IREUnbox TgFun (Lua2Lir Γ e1)) (Lua2Lir Γ e2)
+      IREBox TgFun (IREFun (IRELamb var IRTStar (Lua2Lir body)))
+  | LEApp e1 e2 => IREFunApp (IREUnbox TgFun (Lua2Lir e1)) (Lua2Lir e2)
   end.
-
-
-Definition LuaEnv (Γ : IREnvironment) := forall var T,
-    In Γ var = Some T -> In Γ var = Some IRTStar.
-
-
-Lemma LuaEnvUpdate : forall Γ var, LuaEnv Γ -> LuaEnv (var |=> IRTStar; Γ).
-Proof.
-  unfold LuaEnv.
-  unfold In.
-  intros Γ var HLE var' T HIn.
-  destruct (string_dec var' var); eauto.
-Qed.
 
 
 Inductive LMem : Set :=
 | LEmptyMem : LMem
-| LUpdate : address -> nat -> LE -> LMem -> LMem.
+| LUpdate : address -> Index -> LE -> LMem -> LMem.
 
 
-Fixpoint Lquery (a : address) (idx : nat) (m : LMem) :=
+Axiom LToIndex : LE -> Index.
+
+Axiom LuaIndex : forall e, LToIndex e = ToIndex (Lua2Lir e).
+
+Coercion LToIndex : LE >-> Index.
+
+
+Fixpoint Lquery (a : address) (idx : LE) (m : LMem) :=
   match m with
   | LEmptyMem => LENil
   | LUpdate a' idx' e m' => if Nat.eq_dec a a' then
-                           if Nat.eq_dec idx idx' then e
+                           if Index_dec idx idx' then e
                            else Lquery  a idx m'
                          else Lquery  a idx m'
   end.
@@ -88,7 +93,7 @@ Fixpoint Lfreshaux (m : LMem) : address :=
 
 
 Definition Lfresh (m : LMem) : (address * LMem) :=
-  let f := Lfreshaux m in (f, LUpdate f 1 LENil m).
+  let f := Lfreshaux m in (f, LUpdate f LENil LENil m).
 
 
 Reserved Notation "'[' x ':=' s ']' t" (at level 20, x constr).
@@ -120,85 +125,26 @@ Inductive LValue : LE -> Prop :=
 .
 
 
-Reserved Notation "m '/' e --> m1 '/' e1"
-(at level 40, e at level 39, m1 at level 39, e1 at level 39).
-
-Inductive Lstep : LMem -> LE -> LMem -> LE -> Prop :=
-| LStPlus1 : forall m e1 e2 m' e1',
-    m / e1 --> m' / e1' ->
-    m / LEPlus e1 e2 --> m' / LEPlus e1' e2
-| LStPlus2 : forall m e1 e2 m' e2',
-    LValue e1 ->
-    m / e2 --> m' / e2' ->
-    m /  LEPlus e1 e2 --> m' /  LEPlus e1 e2'
-| LStPlus : forall m n1 n2,
-    m /  LEPlus (LENum n1) (LENum n2) --> m /  LENum (n1 + n2)
-| LStCstr : forall m m' free,
-    (free, m') = Lfresh m ->
-    m / LECnst --> m' / LEAddr free
-| LStGet1 : forall m e1 e2 m' e1',
-    m /e1 --> m' /e1' ->
-    m / LEGet e1 e2 --> m' / LEGet e1' e2
-| LStGet2 : forall m e1 e2 m' e2',
-    LValue e1 ->
-    m /e2 --> m' /e2' ->
-    m / LEGet e1 e2 --> m' / LEGet e1 e2'
-| LStGet : forall m a n,
-    m / LEGet (LEAddr a) (LENum n) --> m / Lquery a n m
-| LStSet1 : forall m e1 e2 e3 m' e1',
-    m / e1 --> m' / e1' ->
-    m / LESet e1 e2 e3 --> m' / LESet e1' e2 e3
-| LStSet2 : forall m e1 e2 e3 m' e2',
-    LValue e1 ->
-    m / e2 --> m' / e2' ->
-    m / LESet e1 e2 e3 --> m' / LESet e1 e2' e3
-| LStSet3 : forall m e1 e2 e3 m' e3',
-    LValue e1 -> LValue e2 ->
-    m / e3 --> m' / e3' ->
-    m / LESet e1 e2 e3 --> m' / LESet e1 e2 e3'
-| LStSet : forall m a n v,
-    LValue v ->
-    m / LESet (LEAddr a) (LENum n) v --> LUpdate a n v m / v
-| LStApp1 : forall m e1 e2 m' e1',
-    m / e1 --> m' / e1' ->
-    m / LEApp e1 e2 --> m' / LEApp e1' e2
-| LStApp2 : forall m e1 e2 m' e2',
-    LValue e1 ->
-    m / e2 --> m' / e2' ->
-    m / LEApp e1 e2 --> m' / LEApp e1 e2'
-| LStApp : forall m var e1 v2,
-     LValue v2 ->
-     m / LEApp (LEFun var e1) v2 -->
-     m / ([var := v2] e1)
-
-where "m / e --> m1 / e1" := (Lstep m e m1 e1)
-.
-
-
-
 (* Issues: 1. globals; 2. type of assignments *)
-Lemma Lua2LirTypeAux : forall Γ e, LuaEnv Γ -> Γ |= Lua2Lir Γ e : IRTStar.
+Lemma Lua2LirTypeAux : forall Γ e, LEWT Γ e -> Γ |= Lua2Lir e : IRTStar.
 Proof.
   intros Γ e.
   generalize dependent Γ.
-  induction e; intros Γ HLE; simpl;
-  try match goal with  |- context [In Γ ?var] =>
-    destruct (In Γ var) eqn:? end;  (* handle variables *)
-  eauto 8 using IRTyping,LuaEnvUpdate.
+  induction e; intros Γ HLE; inversion HLE; subst; simpl;
+  eauto 8 using IRTyping.
 Qed.
 
 
-Lemma LuaIsDyn : forall Γ e, Lua2Lir Γ e = dyn (Lua2Lir Γ e).
+Lemma LuaIsDyn : forall e, Lua2Lir e = dyn (Lua2Lir e).
 Proof.
-  intros Γ e.
-  generalize dependent Γ.
-  induction e; intros Γ; simpl; try congruence.
-  destruct (In Γ s); trivial.
+  intros e.
+  induction e; simpl; try congruence.
 Qed.
 
 
-Corollary Lua2LirType : forall e, MEmpty |= Lua2Lir MEmpty e : IRTStar.
-Proof. intros e. eapply Lua2LirTypeAux. discriminate. Qed.
+Corollary Lua2LirType : forall e,
+    LEWT MEmpty e -> MEmpty |= Lua2Lir e : IRTStar.
+Proof. intros e. eapply Lua2LirTypeAux. Qed.
 
 
 Fixpoint Pall2Lua (e : PE) : LE :=
@@ -214,45 +160,4 @@ Fixpoint Pall2Lua (e : PE) : LE :=
   | PEFun var _ e => LEFun var (Pall2Lua e)
   | PECast e _ => Pall2Lua e
   end.
-
-
-(*
-Ltac destructTag :=
-  simpl;
-  match goal with
-  [ |- context F [tagOf ?C ?E] ] =>
-     idtac C E; destruct (tagOf C E); simpl end.
-
-
-Lemma all : forall Γ e t,
-    PTyping Γ e t ->
-    dyn (Pall2Lir Γ e) = Lua2Lir (TP2TGamma Γ) (Pall2Lua e).
-Proof.
-  intros Γ e.
-  generalize dependent Γ.
-  induction e; intros Γ ? HTy; inversion HTy; subst;
-  repeat match goal with
-  |[ HT : PTyping ?C ?E ?T,
-     IH : forall _, PTyping ?C ?E _ -> _ |- _] =>
-      specialize (IH T HT) end;
-  simpl; try (repeat destructTag; congruence).
-  - repeat match goal with
-   [ HT: PTyping ?G ?E ?T,
-     IH: forall _ _, PTyping _ ?E _ -> _ |- _] =>
-         specialize (IH G T HT)
-     end. congruence.
-  - repeat match goal with
-   [ HT: PTyping ?G ?E ?T,
-     IH: forall _ _, PTyping _ ?E _ -> _ |- _] =>
-         specialize (IH G T HT)
-     end.
-     destructTag; congruence.
-
-  - repeat f_equal. rewrite IHe1.
-  - inversion H1.
-  - destruct (tagOf (s |=> p; MEmpty) e); simpl.
-  - admit.
-Admitted.
-*)
-
 
